Wrote more admitted specs for config and ctr.
Use Coq modules to namespace specs for better naming discipline.

src/program_proof/fencing/config_proof.v
@@ -5,32 +5,67 @@ From Perennial.program_proof.memkv Require Export urpc_lib urpc_proof urpc_spec.
 From Perennial.program_proof.fencing Require Export ctr_proof.
 From iris.base_logic Require Import mono_nat.
 
+Module config.
 Section config_proof.
 Context `{!heapGS Σ}.
 
-Record config_names :=
+Record names :=
   {
 
   }.
 
-Implicit Type γ:config_names.
+Context (γ:names).
 
-Definition is_config_host γ (host:u64) : iProp Σ.
+Definition is_host (host:u64) (epoch_tok : u64 → iProp Σ) (host_inv:u64 → iProp Σ): iProp Σ.
 Admitted.
 
-Definition own_ConfigClerk γ (ck:loc) : iProp Σ.
+Global Instance is_host_pers host epoch_tok host_inv : Persistent (is_host host epoch_tok host_inv).
 Admitted.
 
-Lemma wp_MakeClerk γ host :
-  is_config_host γ host -∗
+Definition is_Clerk (ck:loc) : iProp Σ.
+Admitted.
+
+Global Instance is_Clerk_pers ck : Persistent (is_Clerk ck).
+Admitted.
+
+
+Lemma wp_MakeClerk host epoch_tok host_inv :
+  is_host host epoch_tok host_inv -∗
   {{{
         True
   }}}
     config.MakeClerk #host
   {{{
-        (ck:loc), RET #ck; own_ConfigClerk γ ck
+        (ck:loc), RET #ck; is_Clerk ck
+  }}}.
+Proof.
+Admitted.
+
+Lemma wp_Clerk__AcquireEpoch ck host newHost epoch_tok host_inv :
+  is_host host epoch_tok host_inv -∗
+  is_Clerk ck -∗
+  {{{
+        True
+  }}}
+    config.Clerk__AcquireEpoch #ck #newHost
+  {{{
+        (epoch:u64), RET #epoch; epoch_tok epoch
+  }}}.
+Proof.
+Admitted.
+
+Lemma wp_Clerk__Get ck host epoch_tok host_inv :
+  is_host host epoch_tok host_inv -∗
+  is_Clerk ck -∗
+  {{{
+        True
+  }}}
+    config.Clerk__Get #ck
+  {{{
+        (v:u64), RET #host; host_inv v
   }}}.
 Proof.
 Admitted.
 
 End config_proof.
+End config.
